# Copyright 2020  Platoon Project.
# 
# Licensed under the Apache License, Version 2.0 (the "License");
# you may not use this file except in compliance with the License.
# You may obtain a copy of the License at
# 
#      http://www.apache.org/licenses/LICENSE-2.0
# 
# Unless required by applicable law or agreed to in writing,
# distributed under the License is distributed on an "AS IS" BASIS,
# WITHOUT WARRANTIES OR CONDITIONS OF ANY KIND, either express or implied.
# See the License for the specific language governing permissions and
# limitations under the License.

@prefix rdf: <http://www.w3.org/1999/02/22-rdf-syntax-ns#> .
@prefix owl: <http://www.w3.org/2002/07/owl#> .
@prefix rdfs: <http://www.w3.org/2000/01/rdf-schema#> .
@prefix xsd: <http://www.w3.org/2001/XMLSchema#> .
@prefix dcterms: <http://purl.org/dc/terms/> .
@prefix vann: <http://purl.org/vocab/vann/> .
@prefix voaf: <http://purl.org/vocommons/voaf#> .
@prefix vs: <http://www.w3.org/2003/06/sw-vocab-status/ns#> .
@prefix cc: <http://creativecommons.org/ns#>.
@prefix foaf: <http://xmlns.com/foaf/0.1/>.
@prefix saref: <https://saref.etsi.org/core/> .
@prefix seas: <https://w3id.org/seas/> .
@prefix time: <http://www.w3.org/2006/time#> .
@prefix skos: <http://www.w3.org/2004/02/skos/core#> .
@prefix pep: <https://w3id.org/pep/>.
@prefix cim: <http://ontology.tno.nl/cerise/cim-profile#> .
@prefix fiemser: <http://sites.google.com/site/smartappliancesproject/ontologies/fiemser#> .

@prefix plt: <https://w3id.org/platoon/>.
@base <https://w3id.org/platoon/>.

voaf:Vocabulary a owl:Class .
dcterms:title a owl:AnnotationProperty .
dcterms:description a owl:AnnotationProperty .
dcterms:issued a owl:AnnotationProperty .
dcterms:modified a owl:AnnotationProperty .
dcterms:creator a owl:AnnotationProperty .
dcterms:contributor a owl:AnnotationProperty .
dcterms:license a owl:AnnotationProperty .
vann:preferredNamespacePrefix a owl:AnnotationProperty .
vann:preferredNamespaceUri a owl:AnnotationProperty .
vs:term_status a owl:AnnotationProperty .
foaf:Person a owl:Class .
foaf:name a owl:DatatypeProperty .


plt:EnergyMeasureOntology rdf:type voaf:Vocabulary , owl:Ontology ;
  dcterms:title "Platoon energy ontology"@en ;
  dcterms:description "Links the platoon Energy vocabulary for the  Platoon  project."@en ;
  dcterms:issued "2020-11-17"^^xsd:date ;
  dcterms:modified "2021-07-08"^^xsd:date ;
  dcterms:creator "Sarra BEN ABBES and Lynda TEMAL and Oumy SEYE" ; 
  dcterms:license <https://www.apache.org/licenses/LICENSE-2.0> ;
  vann:preferredNamespacePrefix "plt" ;
  vann:preferredNamespaceUri <https://w3id.org/platoon/> ;  
  owl:versionIRI <https://w3id.org/platoon/EnergyMeasureOntology-1.2> ;
  owl:imports <https://w3id.org/saref> ,   
              seas:ElectricPowerSystemOntology,
              plt:ForecastingOntology,
              seas:SmartMeterOntology;   
  owl:versionInfo "v1.2" .
#######################################
# Energy Consumption                  #
#######################################
plt:EnergyProperty a owl:Class ;
  rdfs:label "Energy  Property"@en ;
  rdfs:comment "The class of properties that are quantifiable and have a quantity kind of energy consumption."@en ;
  owl:equivalentClass saref:Energy;
   rdfs:subClassOf   seas:Property;  
  vs:term_status "testing" ;
  rdfs:isDefinedBy plt:EnergyMeasureOntology .

plt:EnergyEvaluation a owl:Class ;
  rdfs:label "Energy  Evaluation"@en ;
  rdfs:comment """"The class of evaluation for energy properties"""@en ;
  rdfs:subClassOf seas:Evaluation;  
  rdfs:subClassOf [ owl:onProperty seas:evaluationOf ; owl:someValuesFrom plt:EnergyProperty ] ;
  owl:equivalentClass [ owl:onProperty seas:evaluationOf ; owl:someValuesFrom plt:EnergyProperty ] ;
  vs:term_status "testing" ;
  rdfs:isDefinedBy plt:EnergyMeasureOntology .

plt:hasActiveWork a owl:ObjectProperty , owl:FunctionalProperty ;
  rdfs:label "has  active work "@en ;
  rdfs:comment """Link the feature of interest to its  active work."""@en ;
  rdfs:subPropertyOf seas:hasProperty ;
  rdfs:domain seas:FeatureOfInterest ;
  rdfs:range plt:EnergyProperty;
  vs:term_status "testing" ;
  rdfs:isDefinedBy plt:GenericPropertyOntology.

plt:hasNegativeActiveWork a owl:ObjectProperty , owl:FunctionalProperty ;
  rdfs:label "has negative active work "@en ;
  rdfs:comment """Link the feature of interest to its  active work."""@en ;
  rdfs:subPropertyOf plt:hasActiveWork ;
  rdfs:domain seas:FeatureOfInterest ;
  rdfs:range plt:EnergyProperty;
  vs:term_status "testing" ;
  rdfs:isDefinedBy plt:GenericPropertyOntology.

plt:hasPositiveActivework a owl:ObjectProperty , owl:FunctionalProperty ;
  rdfs:label "has  active work "@en ;
  rdfs:comment """Link the feature of interest to its  active work."""@en ;
  rdfs:subPropertyOf plt:hasActiveWork ;
  rdfs:domain seas:FeatureOfInterest ;
  rdfs:range plt:EnergyProperty;
  vs:term_status "testing" ;
  rdfs:isDefinedBy plt:GenericPropertyOntology.

plt:hasReactiveWork a owl:ObjectProperty , owl:FunctionalProperty ;
  rdfs:label "has  reactive work "@en ;
  rdfs:comment """Link the feature of interest to its  active work."""@en ;
  rdfs:subPropertyOf seas:hasProperty ;
  rdfs:domain seas:FeatureOfInterest ;
  rdfs:range plt:EnergyProperty;
  vs:term_status "testing" ;
  rdfs:isDefinedBy plt:GenericPropertyOntology.

plt:hasNegativeReactiveWork a owl:ObjectProperty , owl:FunctionalProperty ;
  rdfs:label "has  active work "@en ;
  rdfs:comment """Link the feature of interest to its  active work."""@en ;
  rdfs:subPropertyOf plt:hasReactiveWork ;
  rdfs:domain seas:FeatureOfInterest ;
  rdfs:range plt:EnergyProperty;
  vs:term_status "testing" ;
  rdfs:isDefinedBy plt:GenericPropertyOntology.

plt:hasPositiveReactiveWork a owl:ObjectProperty , owl:FunctionalProperty ;
  rdfs:label "has  active work "@en ;
  rdfs:comment """Link the feature of interest to its  active work."""@en ;
  rdfs:subPropertyOf plt:hasReactiveWork√í ;
  rdfs:domain seas:FeatureOfInterest ;
  rdfs:range plt:EnergyProperty;
  vs:term_status "testing" ;
  rdfs:isDefinedBy plt:GenericPropertyOntology.

plt:hasLightingEnergyConsumption a owl:ObjectProperty , owl:FunctionalProperty ;
  rdfs:label "has lighting energy consumption"@en ;
  rdfs:comment """Links the feature of interest to its electric energy consumption for lighting."""@en ;
  rdfs:subPropertyOf plt:hasElectricEnergyConsumption ;
  rdfs:domain  seas:FeatureOfInterest ;
  rdfs:range plt:ElectricEnergyConsumptionProperty ;
  vs:term_status "testing" ;
  rdfs:isDefinedBy plt:EnergyMeasureOntology  .

plt:EnergyConsumptionProperty a owl:Class ;
  rdfs:label "Energy  Consumption Property"@en ;
  rdfs:comment "The class of properties that are quantifiable and have a quantity kind of energy consumption."@en ;
  rdfs:subClassOf plt:EnergyProperty,
                  seas:ConsumptionProperty;  
  vs:term_status "testing" ;
  rdfs:isDefinedBy plt:EnergyMeasureOntology .

plt:EnergyConsumptionEvaluation a owl:Class ;
  rdfs:label "Energy  Consumption Evaluation"@en ;
  rdfs:comment "The class of evaluation for energy consumption."@en ;
  rdfs:subClassOf plt:EnergyEvaluation;  
  vs:term_status "testing" ;
  rdfs:isDefinedBy plt:EnergyMeasureOntology .

plt:hasEnergy a owl:ObjectProperty , owl:FunctionalProperty ;
  rdfs:label "has  energy "@en ;
  rdfs:comment """Links the feature of interest to its  energy ."""@en ;
  rdfs:subPropertyOf seas:hasProperty;
  rdfs:domain  seas:FeatureOfInterest ;
  rdfs:range plt:EnergyProperty ;
  vs:term_status "testing" ;
  rdfs:isDefinedBy plt:EnergyMeasureOntology.

plt:hasEnergyConsumption a owl:ObjectProperty , owl:FunctionalProperty ;
  rdfs:label "has  energy consumption"@en ;
  rdfs:comment """Links the feature of interest to its  energy consumption."""@en ;
  rdfs:subPropertyOf seas:consumption,plt:hasEnergy;
  rdfs:domain  seas:FeatureOfInterest ;
  rdfs:range plt:EnergyConsumptionProperty ;
  vs:term_status "testing" ;
  rdfs:isDefinedBy plt:EnergyMeasureOntology  . 

plt:hasSelfEnergyConsumption a owl:ObjectProperty , owl:FunctionalProperty ;
  rdfs:label "has self energy consumption"@en ;
  rdfs:comment """Links the feature of interest to its self energy consumption."""@en ;
  rdfs:subPropertyOf plt:hasEnergyConsumption;
  rdfs:domain  seas:FeatureOfInterest ;
  rdfs:range plt:EnergyConsumptionProperty ;
  vs:term_status "testing" ;
  rdfs:isDefinedBy plt:EnergyMeasureOntology .

plt:ElectricEnergyConsumptionProperty a owl:Class ;
  rdfs:label "Electric Energy Consumption Property"@en ;
  rdfs:comment "The class of properties that are quantifiable and have a quantity kind of electric energy consumption."@en ;
  rdfs:subClassOf seas:ElectricEnergyProperty;
  rdfs:subClassOf plt:EnergyConsumptionProperty;  
  vs:term_status "testing" ;
  rdfs:isDefinedBy plt:EnergyMeasureOntology .

plt:ElectricEnergyConsumptionEvaluation a owl:Class ;
  rdfs:label "Electric Energy Consumption Evaluation"@en ;
  rdfs:comment """"The class of evaluation for electric energy consumption properties"""@en ;
  rdfs:subClassOf seas:ElectricEnergyEvaluation;  
  rdfs:subClassOf [ owl:onProperty seas:evaluationOf ; owl:someValuesFrom plt:ElectricEnergyConsumptionProperty ] ;
  owl:equivalentClass [ owl:onProperty seas:evaluationOf ; owl:someValuesFrom plt:ElectricEnergyConsumptionProperty ] ;
  vs:term_status "testing" ;
  rdfs:isDefinedBy plt:EnergyMeasureOntology .

plt:hasEstimatedLightingEnergyConsumption a owl:ObjectProperty , owl:FunctionalProperty ;
  rdfs:label "has estimated lighting energy consumption"@en ;
  rdfs:comment """Links the feature of interest to its estimated electric energy consumption for lighting."""@en ;
  rdfs:subPropertyOf plt:hasLightingEnergyConsumption ;
  rdfs:domain  seas:FeatureOfInterest ;
  rdfs:range plt:ElectricEnergyConsumptionProperty ;
  vs:term_status "testing" ;
  rdfs:isDefinedBy plt:EnergyMeasureOntology  .

plt:hasElectricEnergyConsumption a owl:ObjectProperty , owl:FunctionalProperty ;
  rdfs:label "has electric energy consumption"@en ;
  rdfs:comment """Links the feature of interest to its electric energy consumption ."""@en ;
  rdfs:subPropertyOf plt:hasEnergyConsumption;
  rdfs:domain  seas:FeatureOfInterest ;
  rdfs:range plt:ElectricEnergyConsumptionProperty ;
  vs:term_status "testing" ;
  rdfs:isDefinedBy plt:EnergyMeasureOntology  .

plt:HeatingElectricEnergyConsumptionProperty a owl:Class ;
  rdfs:label "Heating Electric Energy Consumption Property"@en ;
  rdfs:comment "The class of properties that are quantifiable and have a quantity kind of electric energy consumption for heating."@en ;
  rdfs:subClassOf plt:ElectricEnergyConsumptionProperty,plt:ThermalEnergyProperty;  
  vs:term_status "testing" ;
  rdfs:isDefinedBy plt:EnergyMeasureOntology .

plt:HeatingElectricEnergyConsumptionEvaluation a owl:Class ;
  rdfs:label "Heating Electric Energy Consumption Evaluation"@en ;
  rdfs:comment "The class of evaluation for heating energy consumption properties"@en ;
  rdfs:subClassOf plt:ElectricEnergyConsumptionEvaluation;  
  owl:equivalentClass [ owl:onProperty seas:evaluationOf ; owl:someValuesFrom plt:HeatingElectricEnergyConsumptionProperty ] ;
  vs:term_status "testing" ;
  rdfs:isDefinedBy plt:EnergyMeasureOntology .

plt:hasHeatingElectricEnergyConsumption a owl:ObjectProperty , owl:FunctionalProperty ;
  rdfs:label "has Heating Electric Energy Consumption"@en ;
  rdfs:comment """Links the feature of interest to its heating electric energy consumption."""@en ;
  rdfs:subPropertyOf plt:hasElectricEnergyConsumption ;
  rdfs:domain seas:FeatureOfInterest;
  rdfs:range plt:HeatingElectricEnergyConsumptionProperty ;
  vs:term_status "testing" ;
  rdfs:isDefinedBy plt:EnergyMeasureOntology  .

plt:DomesticHotWaterElectricEnergyConsumptionProperty a owl:Class ;
  rdfs:label "Domestic Hot Water Electric Energy Consumption Property"@en ;
  rdfs:comment "The class of properties that are quantifiable and have a quantity kind of domestic hot water electric energy consumption property"@en ;
  rdfs:subClassOf plt:ElectricEnergyConsumptionProperty;  
  vs:term_status "testing" ;
  rdfs:isDefinedBy plt:EnergyMeasureOntology .

plt:DomesticHotWaterElectricEnergyConsumptionEvaluation a owl:Class ;
  rdfs:label "Heating Electric Energy Consumption Evaluation"@en ;
  rdfs:comment "The class of evaluation for domestic hot water electric energy consumption properties"@en ;
  rdfs:subClassOf plt:ElectricEnergyConsumptionEvaluation;  
  owl:equivalentClass [ owl:onProperty seas:evaluationOf ; owl:someValuesFrom plt:DomesticHotWaterElectricEnergyConsumptionProperty ] ;
  vs:term_status "testing" ;
  rdfs:isDefinedBy plt:EnergyMeasureOntology .

plt:hasDomesticHotWaterElectricEnergyConsumption a owl:ObjectProperty , owl:FunctionalProperty ;
  rdfs:label "has domestic hot water electric energy consumption"@en ;
  rdfs:comment """Links the feature of interest to its domestic hot water electric energy consumption."""@en ;
  rdfs:subPropertyOf plt:hasElectricEnergyConsumption ;
  rdfs:domain seas:FeatureOfInterest ;
  rdfs:range plt:DomesticHotWaterElectricEnergyConsumptionProperty ;
  vs:term_status "testing" ;
  rdfs:isDefinedBy plt:EnergyMeasureOntology.

plt:CoolingElectricEnergyConsumptionProperty a owl:Class ;
  rdfs:label "Cooling Energy Consumption Property"@en ;
  rdfs:comment "The class of properties that are quantifiable and have a quantity kind of electric energy consumption for cooling"@en ;
  rdfs:subClassOf plt:ElectricEnergyConsumptionProperty;  
  vs:term_status "testing" ;
  rdfs:isDefinedBy plt:EnergyMeasureOntology .

plt:CoolingElectricEnergyConsumptionEvaluation a owl:Class ;
  rdfs:label "Cooling Electric Energy Consumption Evaluation"@en ;
  rdfs:comment "The class of evaluation for cooling energy consumption properties"@en ;
  rdfs:subClassOf plt:ElectricEnergyConsumptionEvaluation;    
  rdfs:subClassOf [ a owl:Restriction ; owl:onProperty seas:evaluationOf ; owl:someValuesFrom plt:CoolingElectricEnergyConsumptionProperty ] ;
  rdfs:subClassOf [ a owl:Restriction ; owl:onProperty seas:evaluatedSimpleValue; owl:someValuesFrom  xsd:decimal] ;
  owl:equivalentClass [ owl:onProperty seas:evaluationOf ; owl:someValuesFrom plt:CoolingElectricEnergyConsumptionProperty ] ;
  vs:term_status "testing" ;
  rdfs:isDefinedBy plt:EnergyMeasureOntology .

plt:hasCoolingEnergyConsumption a owl:ObjectProperty , owl:FunctionalProperty ;
  rdfs:label "has cooling electric energy consumption"@en ;
  rdfs:comment """Links the feature of interest to its climate corrected cooling electric energy consumption ."""@en ;
  rdfs:subPropertyOf plt:hasEnergyConsumption ;
  rdfs:domain seas:FeatureOfInterest;
  rdfs:range plt:CoolingElectricEnergyConsumptionProperty ;
  vs:term_status "testing" ;
  rdfs:isDefinedBy plt:EnergyMeasureOntology  .

plt:hasCoolingElectricEnergyConsumption a owl:ObjectProperty , owl:FunctionalProperty ;
  rdfs:label "has cooling electric energy consumption"@en ;
  rdfs:comment """Links the feature of interest to its cooling electric energy consumption ."""@en ;
  rdfs:subPropertyOf plt:hasElectricEnergyConsumption, plt:hasCoolingEnergyConsumption;
  rdfs:domain seas:FeatureOfInterest;
  rdfs:range plt:CoolingElectricEnergyConsumptionProperty ;
  vs:term_status "testing" ;
  rdfs:isDefinedBy plt:EnergyMeasureOntology  .

plt:hasClimateCorrectedCoolingEnergyConsumption a owl:ObjectProperty , owl:FunctionalProperty ;
  rdfs:label "has climate corrected cooling  energy consumption"@en ;
  rdfs:comment """Links the feature of interest to its climate corrected cooling  energy consumption ."""@en ;
  rdfs:subPropertyOf plt:hasCoolingEnergyConsumption ;
  rdfs:domain seas:FeatureOfInterest;
  rdfs:range plt:CoolingEnergyConsumptionProperty ;
  vs:term_status "testing" ;
  rdfs:isDefinedBy plt:EnergyMeasureOntology  .

plt:ForecastOfEnergyProperty a owl:Class ;
  rdfs:label "Forecast Of Energy Property"@en ;
  rdfs:comment "The class for forecast of energy  properties"@en ;
  rdfs:subClassOf seas:Forecast; 
  rdfs:subClassOf[ owl:onProperty seas:forecastsProperty ; owl:someValuesFrom plt:EnergyProperty ] ;
  vs:term_status "testing" ;
  rdfs:isDefinedBy plt:EnergyMeasureOntology .

plt:ForecastOfEnergyConsumptionProperty a owl:Class ;
  rdfs:label "Forecast Of Energy Consumption Property"@en ;
  rdfs:comment "The class for forecast of energy consumption properties"@en ;
  rdfs:subClassOf plt:ForecastOfEnergyProperty; 
  rdfs:subClassOf[ owl:onProperty seas:forecastsProperty ; owl:someValuesFrom plt:EnergyConsumptionProperty ] ;
  vs:term_status "testing" ;
  rdfs:isDefinedBy plt:EnergyMeasureOntology .

plt:hasForecastOfEnergyConsumptionProperty a owl:ObjectProperty , owl:FunctionalProperty ;
  rdfs:label "has forecast of energy consumption property"@en ;
  rdfs:comment """Links the feature of interest to its forecast of energy consumption property."""@en ;
  rdfs:subPropertyOf plt:hasForecastOfProperty ;
  rdfs:domain seas:FeatureOfInterest ;
  rdfs:range plt:ForecastOfEnergyConsumptionProperty ;
  vs:term_status "testing" ;
  rdfs:isDefinedBy plt:EnergyMeasureOntology .

plt:ForecastOfCoolingElectricEnergyConsumptionProperty a owl:Class ;
  rdfs:label "Forecast Of Cooling Electric Energy Consumption Property"@en ;
  rdfs:comment "The class for forecast of cooling Electric energy consumption properties"@en ;
  rdfs:subClassOf plt:ForecastOfEnergyConsumptionProperty; 
  rdfs:subClassOf[ owl:onProperty seas:forecastsProperty ; owl:someValuesFrom plt:CoolingElectricEnergyConsumptionProperty ] ;
  rdfs:subClassOf[ owl:onProperty pep:hasResult ; owl:someValuesFrom owl:individual ] ;
  vs:term_status "testing" ;
  rdfs:isDefinedBy plt:EnergyMeasureOntology .

plt:hasForecastOfCoolingElectricEnergyConsumptionProperty a owl:ObjectProperty , owl:FunctionalProperty ;
  rdfs:label "has forecast Cooling Electric Energy Consumption Property"@en ;
  rdfs:comment """Links the feature of interest to its forecast of electric energy consumption property ."""@en ;
  rdfs:subPropertyOf plt:hasForecastOfEnergyConsumptionProperty,plt:hasForecastOfElectricEnergyProperty;
  rdfs:domain seas:FeatureOfInterest;
  rdfs:range plt:ForecastOfCoolingElectricEnergyConsumptionProperty ;
  vs:term_status "testing" ;
  rdfs:isDefinedBy plt:EnergyMeasureOntology .

plt:ForecastOfHeatingElectricEnergyConsumptionProperty a owl:Class ;
  rdfs:label "Forecast Of Heating Electric Energy Consumption Property"@en ;
  rdfs:comment "The class for forecast of  heating Electric energy consumption properties"@en ;
  rdfs:subClassOf plt:ForecastOfEnergyConsumptionProperty; 
  rdfs:subClassOf[ owl:onProperty seas:forecastsProperty ; owl:someValuesFrom plt:HeatingElectricEnergyConsumptionProperty ] ;
  rdfs:subClassOf[ owl:onProperty pep:hasResult ; owl:someValuesFrom owl:individual ] ;
  vs:term_status "testing" ;
  rdfs:isDefinedBy plt:EnergyMeasureOntology .

plt:hasForecastOfHeatingElectricEnergyConsumptionProperty a owl:ObjectProperty , owl:FunctionalProperty ;
  rdfs:label "has forecast of heating electric energy consumption property"@en ;
  rdfs:comment """Links the feature of interest to its forecast of electric energy consumption property."""@en ;
  rdfs:subPropertyOf plt:hasForecastOfEnergyConsumptionProperty,plt:hasForecastOfElectricEnergyProperty;
  rdfs:domain seas:FeatureOfInterest ;
  rdfs:range plt:ForecastOfHeatingElectricEnergyConsumptionProperty ,plt:hasForecastOfElectricEnergyProperty;
  vs:term_status "testing" ;
  rdfs:isDefinedBy plt:EnergyMeasureOntology .

#######################################
# thermmal energy Consumption         #
#######################################
plt:ThermalEnergyConsumptionProperty a owl:Class ;
  rdfs:label "Thermal Energy Consumption Property"@en ;
  skos:altLabel "ThermalEnergy";
  rdfs:comment "The class of properties that are quantifiable and have a quantity kind of thermmal energy consumption"@en ;
  rdfs:subClassOf plt:EnergyConsumptionProperty, plt:ThermalEnergyProperty ;
  vs:term_status "testing" ;
  rdfs:isDefinedBy plt:EnergyMeasureOntology .

plt:ThermalEnergyConsumptionEvaluation a owl:Class ;
  rdfs:label "Thermal Energy Consumption Evaluation"@en ;
  rdfs:comment "The class of evaluation for thermmal energy consumption properties"@en ;
  rdfs:subClassOf plt:EnergyEvaluation;  
  rdfs:subClassOf [ a owl:Restriction ; owl:onProperty seas:evaluationOf ; owl:someValuesFrom plt:ThermalEnergyConsumptionProperty ] ;
  rdfs:subClassOf [ a owl:Restriction ; owl:onProperty seas:evaluatedSimpleValue; owl:someValuesFrom  xsd:decimal] ;
  owl:equivalentClass [ owl:onProperty seas:evaluationOf ; owl:someValuesFrom plt:ThermalEnergyConsumptionProperty ] ;
  vs:term_status "testing" ;
  rdfs:isDefinedBy plt:EnergyMeasureOntology .

plt:hasThermalEnergyConsumption a owl:ObjectProperty , owl:FunctionalProperty ;
  rdfs:label "has thermmal energy consumption"@en ;
  rdfs:comment """Links the feature of interest to its thermmal energy consumption property."""@en ;
  rdfs:subPropertyOf plt:hasEnergyConsumption ;
  rdfs:domain seas:FeatureOfInterest ;
  rdfs:range plt:ThermalEnergyConsumptionProperty ;
  vs:term_status "testing" ;
  rdfs:isDefinedBy plt:EnergyMeasureOntology.

#######################################
# Gas energy Consumption              #
#######################################

plt:GasEnergyProperty a owl:Class ;
  rdfs:label "Gas  energy Property"@en ;
  rdfs:comment "The class of properties that are quantifiable and have a quantity kind of gas energy "@en ;
  rdfs:subClassOf plt:EnergyProperty;
  vs:term_status "testing" ;
  rdfs:isDefinedBy plt:EnergyMeasureOntology .

plt:GasEnergyEvaluation a owl:Class ;
  rdfs:label " Gas Energy Evaluation"@en ;
  rdfs:comment "The class of evaluation for  gas energy  properties"@en ;
  rdfs:subClassOf plt:EnergyEvaluation;  
  rdfs:subClassOf [ a owl:Restriction ; owl:onProperty seas:evaluationOf ; owl:someValuesFrom plt:GasEnergyProperty ] ;
  owl:equivalentClass [ owl:onProperty seas:evaluationOf ; owl:someValuesFrom plt:GasEnergyProperty ] ;
  vs:term_status "testing" ;
  rdfs:isDefinedBy plt:EnergyMeasureOntology .

plt:GasEnergyConsumptionProperty a owl:Class ;
  rdfs:label "Gas Energy Consumption Property"@en ;
  rdfs:comment "The class of properties that are quantifiable and have a quantity kind of gas energy consumption "@en ;
  rdfs:subClassOf plt:GasEnergyProperty,plt:EnergyConsumptionProperty ;
  vs:term_status "testing" ;
  rdfs:isDefinedBy plt:EnergyMeasureOntology .

plt:GasEnergyConsumptionEvaluation a owl:Class ;
  rdfs:label " Gas Energy Consumption Evaluation"@en ;
  rdfs:comment "The class of evaluation for  gas energy  properties"@en ;
  rdfs:subClassOf plt:GasEnergyEvaluation;  
  rdfs:subClassOf [ a owl:Restriction ; owl:onProperty seas:evaluationOf ; owl:someValuesFrom plt:GasEnergyProperty ] ;
  owl:equivalentClass [ owl:onProperty seas:evaluationOf ; owl:someValuesFrom plt:GasEnergyProperty ] ;
  vs:term_status "testing" ;
  rdfs:isDefinedBy plt:EnergyMeasureOntology .

plt:hasGasEnergyConsumption a owl:ObjectProperty , owl:FunctionalProperty ;
  rdfs:label "has gas energy consumption"@en ;
  rdfs:comment """Links the feature of interest to its gas energy consumption property."""@en ;
  rdfs:subPropertyOf plt:hasEnergyConsumption ;
  rdfs:domain seas:FeatureOfInterest ;
  rdfs:range plt:GasEnergyConsumptionProperty ;
  vs:term_status "testing" ;
  rdfs:isDefinedBy plt:EnergyMeasureOntology.

plt:hasTotalGasEnergyConsumption a owl:ObjectProperty , owl:FunctionalProperty ;
  rdfs:label "has total gas energy consumption"@en ;
  rdfs:comment """Links the feature of interest to its total gas energy consumption property."""@en ;
  rdfs:subPropertyOf plt:hasGasEnergyConsumption ;
  rdfs:domain seas:FeatureOfInterest ;
  rdfs:range plt:GasEnergyConsumptionProperty ;
  vs:term_status "testing" ;
  rdfs:isDefinedBy plt:EnergyMeasureOntology.

plt:HeatingGasEnergyConsumptionProperty a owl:Class ;
  rdfs:label "Heating Gas Energy Consumption Property"@en ;
  rdfs:comment "The class of properties that are quantifiable and have a quantity kind of gas energy consumption for heating"@en ;
  rdfs:subClassOf plt:GasEnergyConsumptionProperty ;
  vs:term_status "testing" ;
  rdfs:isDefinedBy plt:EnergyMeasureOntology .

plt:HeatingGasEnergyConsumptionEvaluation a owl:Class ;
  rdfs:label "Heating Gas Energy Consumption Evaluation"@en ;
  rdfs:comment "The class of evaluation for heating gas energy consumption properties"@en ;
  rdfs:subClassOf plt:GasEnergyConsumptionEvaluation;  
  rdfs:subClassOf [ a owl:Restriction ; owl:onProperty seas:evaluationOf ; owl:someValuesFrom plt:HeatingGasEnergyConsumptionProperty ] ;
  owl:equivalentClass [ owl:onProperty seas:evaluationOf ; owl:someValuesFrom plt:HeatingGasEnergyConsumptionProperty ] ;
  vs:term_status "testing" ;
  rdfs:isDefinedBy plt:EnergyMeasureOntology .

plt:hasHeatingGasEnergyConsumption a owl:ObjectProperty , owl:FunctionalProperty ;
  rdfs:label "has heating gas energy consumption"@en ;
  rdfs:comment """Links the feature of interest to its heating gas energy consumption property."""@en ;
  rdfs:subPropertyOf plt:hasGasEnergyConsumption ;
  rdfs:domain seas:FeatureOfInterest ;
  rdfs:range plt:HeatingGasEnergyConsumptionProperty ;
  vs:term_status "testing" ;
  rdfs:isDefinedBy plt:EnergyMeasureOntology.

plt:CoolingGasEnergyConsumptionProperty a owl:Class ;
  rdfs:label "Cooling Gas Energy Consumption Property"@en ;
  rdfs:comment "The class of properties that are quantifiable and have a quantity kind of cooling gas energy consumption for heating"@en ;
  rdfs:subClassOf plt:GasEnergyConsumptionProperty ;
  vs:term_status "testing" ;
  rdfs:isDefinedBy plt:EnergyMeasureOntology .

plt:CoolingGasEnergyConsumptionEvaluation a owl:Class ;
  rdfs:label "Cooling Gas Energy Consumption Evaluation"@en ;
  rdfs:comment "The class of evaluation for heating gas energy consumption properties"@en ;
  rdfs:subClassOf plt:GasEnergyConsumptionEvaluation;  
  rdfs:subClassOf [ a owl:Restriction ; owl:onProperty seas:evaluationOf ; owl:someValuesFrom plt:HeatingGasEnergyConsumptionProperty ] ;
  owl:equivalentClass [ owl:onProperty seas:evaluationOf ; owl:someValuesFrom plt:HeatingGasEnergyConsumptionProperty ] ;
  vs:term_status "testing" ;
  rdfs:isDefinedBy plt:EnergyMeasureOntology .

plt:hasCoolingGasEnergyConsumption a owl:ObjectProperty , owl:FunctionalProperty ;
  rdfs:label "has Cooling gas energy consumption"@en ;
  rdfs:comment """Links the feature of interest to its cooling gas energy consumption property."""@en ;
  rdfs:subPropertyOf plt:hasGasEnergyConsumption ;
  rdfs:domain seas:FeatureOfInterest ;
  rdfs:range plt:CoolingGasEnergyConsumptionProperty ;
  vs:term_status "testing" ;
  rdfs:isDefinedBy plt:EnergyMeasureOntology.

plt:DomesticHotWaterGasEnergyConsumptionProperty a owl:Class ;
  rdfs:label "Domestic Hot Water Gas Energy Consumption Property"@en ;
  rdfs:comment "The class of properties that are quantifiable and have a quantity kind of domestic hot water gas energy consumption property"@en ;
  rdfs:subClassOf plt:GasEnergyConsumptionProperty;  
  vs:term_status "testing" ;
  rdfs:isDefinedBy plt:EnergyMeasureOntology .

plt:DomesticHotWaterGasEnergyConsumptionEvaluation a owl:Class ;
  rdfs:label "Heating Gas Energy Consumption Evaluation"@en ;
  rdfs:comment "The class of evaluation for domestic hot water gas energy consumption properties"@en ;
  rdfs:subClassOf plt:GasEnergyConsumptionEvaluation;  
  owl:equivalentClass [ owl:onProperty seas:evaluationOf ; owl:someValuesFrom plt:DomesticHotWaterElectricEnergyConsumptionProperty ] ;
  vs:term_status "testing" ;
  rdfs:isDefinedBy plt:EnergyMeasureOntology .

plt:hasDomesticHotWaterGasEnergyConsumption a owl:ObjectProperty , owl:FunctionalProperty ;
  rdfs:label "has domestic hot water gas energy consumption"@en ;
  rdfs:comment """Links the feature of interest to its domestic hot water gas energy consumption."""@en ;
  rdfs:subPropertyOf plt:hasGasEnergyConsumption ;
  rdfs:domain seas:FeatureOfInterest ;
  rdfs:range plt:DomesticHotWaterGasEnergyConsumptionProperty ;
  vs:term_status "testing" ;
  rdfs:isDefinedBy plt:EnergyMeasureOntology.
#######################################
# Energy Production                   #
#######################################
plt:EnergyProductionProperty a owl:Class ;
  rdfs:label "Energy Production Property"@en ;
  rdfs:comment "The class of properties that are quantifiable and have a quantity kind of  energy production."@en ;
  rdfs:subClassOf plt:EnergyProperty,
                  seas:ProductionProperty;  
  vs:term_status "testing" ;
  rdfs:isDefinedBy plt:EnergyMeasureOntology .


plt:EnergyProductionEvaluation a owl:Class ;
  rdfs:label "Energy Production Evaluation"@en ;
  rdfs:comment "The class of evaluation for  energy production properties"@en ;
  rdfs:subClassOf seas:Evaluation;  
  rdfs:subClassOf [ a owl:Restriction ; owl:onProperty seas:evaluationOf ; owl:someValuesFrom plt:EnergyProductionProperty ] ;
  owl:equivalentClass [ owl:onProperty seas:evaluationOf ; owl:someValuesFrom plt:EnergyProductionProperty ] ;
  vs:term_status "testing" ;
  rdfs:isDefinedBy plt:EnergyMeasureOntology .

plt:hasEnergyProduction a owl:ObjectProperty , owl:FunctionalProperty ;
  rdfs:label "has energy production"@en ;
  rdfs:comment """Links the FeatureOfInterest to its energy production property."""@en ;
  rdfs:subPropertyOf seas:production ;
  rdfs:domain seas:FeatureOfInterest ;
  rdfs:range plt:EnergyProductionProperty;
  vs:term_status "testing" ;
  rdfs:isDefinedBy plt:EnergyMeasureOntology  .

plt:ElectricEnergyProductionProperty a owl:Class ;
  rdfs:label "Electric Energy Production Property"@en ;
  rdfs:comment """The class of properties that are quantifiable and have a quantity kind electric energy production."""@en ;
  rdfs:subClassOf plt:EnergyProductionProperty ,
                  seas:ElectricEnergyProperty;  
  vs:term_status "testing" ;
  rdfs:isDefinedBy plt:EnergyMeasureOntology .

plt:ElectricEnergyProductionEvaluation a owl:Class ;
  rdfs:label "Electric Energy Production Evaluation"@en ;
  rdfs:comment "The class of evaluation for electric energy production  properties"@en ;
  rdfs:subClassOf seas:ElectricEnergyEvaluation,plt:EnergyProductionEvaluation;    
  owl:equivalentClass [ owl:onProperty seas:evaluationOf ; owl:someValuesFrom plt:ElectricEnergyProductionProperty ] ;
  vs:term_status "testing" ;
  rdfs:isDefinedBy plt:EnergyMeasureOntology .


plt:PhotovoltaicEnergyProductionProperty a owl:Class ;
  rdfs:label "Photovoltaic Energy Production Property"@en ;
  rdfs:comment "The class of properties that are quantifiable and have a quantity kind of photovoltaic energy production."@en ;
  rdfs:subClassOf plt:EnergyProductionProperty;  
  vs:term_status "testing" ;
  rdfs:isDefinedBy plt:EnergyMeasureOntology .

plt:PhotovoltaicEnergyProductionEvaluation a owl:Class ;
  rdfs:label "Photovoltaic Energy Production Evaluation"@en ;
  rdfs:comment """"The class of evaluation for photovoltaic energy production properties"""@en ;
  rdfs:subClassOf plt:EnergyProductionEvaluation;  
  rdfs:subClassOf [ a owl:Restriction ; owl:onProperty seas:evaluationOf ; owl:someValuesFrom plt:PhotovoltaicEnergyProductionProperty ] ;
  owl:equivalentClass [ owl:onProperty seas:evaluationOf ; owl:someValuesFrom plt:PhotovoltaicEnergyProductionProperty ] ;
  vs:term_status "testing" ;
  rdfs:isDefinedBy plt:EnergyMeasureOntology .

plt:hasPhotovoltaicEnergyProduction a owl:ObjectProperty , owl:FunctionalProperty ;
  rdfs:label "has Photovoltaic energy Production"@en ;
  rdfs:comment """Links the FeatureOfInterest to its photovoltaic energy production."""@en ;
  rdfs:subPropertyOf plt:hasEnergyProduction ;
  rdfs:domain seas:FeatureOfInterest ;
  rdfs:range plt:PhotovoltaicEnergyProductionProperty ;
  vs:term_status "testing" ;
  rdfs:isDefinedBy plt:EnergyMeasureOntology  .

plt:ForecastOfPhotovoltaicEnergyProductionProperty a owl:Class ;
  rdfs:label "Forecast Of Photovoltaic Energy Production Property"@en ;
  rdfs:comment "The class for forecast of photovoltaic energy production properties"@en ;
  rdfs:subClassOf plt:ForecastOfEnergyProperty; 
  rdfs:subClassOf[ owl:onProperty seas:forecastsProperty ; owl:someValuesFrom plt:PhotovoltaicEnergyProductionProperty ] ;
  vs:term_status "testing" ;
  rdfs:isDefinedBy plt:EnergyMeasureOntology .

plt:hasForecastOfPhotovoltaicEnergyProductionProperty a owl:ObjectProperty , owl:FunctionalProperty ;
  rdfs:label "has forecast of photovoltaic energy production property"@en ;
  rdfs:comment """Links the FeatureOfInterest to its forecast of photovoltaic energy production."""@en ;
  rdfs:subPropertyOf plt:hasForecastOfProperty ;
  rdfs:domain seas:FeatureOfInterest: ;
  rdfs:range plt:ForecastOfPhotovoltaicEnergyProductionProperty ;
  vs:term_status "testing" ;
  rdfs:isDefinedBy plt:EnergyMeasureOntology .

#######################################
# Power                 #
#######################################
plt:ForecastOfElectricPowerProperty a owl:Class ;
  rdfs:label "Forecast Of Photovoltaic Electric Power Property"@en ;
  rdfs:comment "The class for forecast of  electric power properties"@en ;
  rdfs:subClassOf seas:Forecast; 
  rdfs:subClassOf[ owl:onProperty seas:forecastsProperty ; owl:someValuesFrom seas:ElectricPowerProperty ] ;
  vs:term_status "testing" ;
  rdfs:isDefinedBy plt:EnergyMeasureOntology .

plt:hasForecastOfElectricPowerProperty a owl:ObjectProperty , owl:FunctionalProperty ;
  rdfs:label "has forecast of electric power property"@en ;
  rdfs:comment """Links the FeatureOfInterest to its forecast of electric power."""@en ;
  rdfs:subPropertyOf plt:hasForecastOfProperty ;
  rdfs:domain seas:FeatureOfInterest: ;
  rdfs:range plt:ForecastOfElectricPowerProperty ;
  vs:term_status "testing" ;
  rdfs:isDefinedBy plt:EnergyMeasureOntology .

plt:hasForecastOfPowerProduction a owl:ObjectProperty , owl:FunctionalProperty ;
  rdfs:label "has forecast of electric power production property"@en ;
  rdfs:comment """Links the FeatureOfInterest to its forecast of electric power production."""@en ;
  rdfs:subPropertyOf plt:hasForecastOfProperty;
  rdfs:domain seas:FeatureOfInterest: ;
  rdfs:range plt:ForecastOfElectricPowerProperty ;
  vs:term_status "testing" ;
  rdfs:isDefinedBy plt:EnergyMeasureOntology .

plt:hasOutputPower a owl:ObjectProperty , owl:FunctionalProperty ;
  rdfs:label "has output  power"@en ;
  rdfs:comment """Links the feature of interest to its output  power."""@en ;
  rdfs:subPropertyOf seas:electricPower ;
  rdfs:domain seas:FeatureOfInterest ;
  rdfs:range seas:ElectricPowerProperty ;
  vs:term_status "testing" ;
  rdfs:isDefinedBy plt:EnergyMeasureOntology.

plt:hasOutputActivePower a owl:ObjectProperty , owl:FunctionalProperty ;
  rdfs:label "has output active power"@en ;
  rdfs:comment """Links the feature of interest to its output active power."""@en ;
  rdfs:subPropertyOf plt:hasOutputPower , seas:activePower;
  rdfs:domain seas:FeatureOfInterest ;
  rdfs:range seas:ElectricPowerProperty ;
  vs:term_status "testing" ;
  rdfs:isDefinedBy plt:EnergyMeasureOntology.

plt:hasRatedePower a owl:ObjectProperty , owl:FunctionalProperty ;
  rdfs:label "has rated power"@en ;
  rdfs:comment """Links the feature of interest to its rated power."""@en ;
  rdfs:subPropertyOf seas:electricPower;
  rdfs:domain seas:FeatureOfInterest ;
  rdfs:range seas:ElectricPowerProperty ;
  vs:term_status "testing" ;
  rdfs:isDefinedBy plt:EnergyMeasureOntology.

plt:hasInputActivePower a owl:ObjectProperty , owl:FunctionalProperty ;
  rdfs:label "has input active power"@en ;
  rdfs:comment """Links the feature of interest to its input active power."""@en ;
  rdfs:subPropertyOf plt:hasInputPower, seas:activePower ;
  rdfs:domain seas:FeatureOfInterest ;
  rdfs:range seas:ElectricPowerProperty ;
  vs:term_status "testing" ;
  rdfs:isDefinedBy plt:EnergyMeasureOntology.

plt:hasReactiveOutputPower a owl:ObjectProperty , owl:FunctionalProperty ;
  rdfs:label "has reactive output power"@en ;
  rdfs:comment """Links the feature of interest to its output reactive power."""@en ;
  rdfs:subPropertyOf plt:hasOutputPower,seas:reactivePower ;
  rdfs:domain seas:FeatureOfInterest ;
  rdfs:range seas:ElectricPowerProperty ;
  vs:term_status "testing" ;
  rdfs:isDefinedBy plt:EnergyMeasureOntology.

plt:hasOutputApparentPower a owl:ObjectProperty , owl:FunctionalProperty ;
  rdfs:label "has output apparent  power"@en ;
  rdfs:comment """Links the feature of interest to its output apparent power."""@en ;
  rdfs:subPropertyOf plt:hasOutputPower,seas:apparentPower ;
  rdfs:domain seas:FeatureOfInterest ;
  rdfs:range seas:ElectricPowerProperty ;
  vs:term_status "testing" ;
  rdfs:isDefinedBy plt:EnergyMeasureOntology.

plt:hasNominalPower a owl:ObjectProperty , owl:FunctionalProperty ;
  rdfs:label "has nominal power"@en ;
  rdfs:comment """Links the feature of interest to its nominal power."""@en ;
  owl:equivalentProperty fiemser:hasNominalPower ;
  rdfs:subPropertyOf seas:hasProperty ;
  rdfs:domain seas:FeatureOfInterest ;
  rdfs:range seas:ElectricPowerProperty ;
  vs:term_status "testing" ;
  rdfs:isDefinedBy plt:EnergyMeasureOntology.

plt:hasInputPower a owl:ObjectProperty , owl:FunctionalProperty ;
  rdfs:label "has input power"@en ;
  rdfs:comment """Links the feature of interest to its input power."""@en ;
  rdfs:subPropertyOf seas:electricPower;
  rdfs:domain seas:FeatureOfInterest ;
  rdfs:range seas:ElectricPowerProperty ;
  vs:term_status "testing" ;
  rdfs:isDefinedBy plt:EnergyMeasureOntology.

plt:hasPowerProduction a owl:ObjectProperty , owl:FunctionalProperty ;
  rdfs:label "has power production"@en ;
  rdfs:comment """Links the feature of interest to its power production."""@en ;
  rdfs:subPropertyOf seas:electricPower,seas:production ;
  rdfs:domain seas:FeatureOfInterest ;
  rdfs:range seas:ElectricPowerProperty ;
  vs:term_status "testing" ;
  rdfs:isDefinedBy plt:EnergyMeasureOntology.


plt:hasActivePowerProduction a owl:ObjectProperty , owl:FunctionalProperty ;
  rdfs:label "has active power production"@en ;
  rdfs:comment """Links the feature of interest to its active power production."""@en ;
  rdfs:subPropertyOf plt:hasPowerProduction , seas:activePower;
  rdfs:domain seas:FeatureOfInterest ;
  rdfs:range seas:ElectricPowerProperty ;
  vs:term_status "testing" ;
  rdfs:isDefinedBy plt:EnergyMeasureOntology.

plt:hasReactivePowerProduction a owl:ObjectProperty , owl:FunctionalProperty ;
  rdfs:label "has reactive power production"@en ;
  rdfs:comment """Links the feature of interest to its reactive power production."""@en ;
  rdfs:subPropertyOf plt:hasPowerProduction , seas:reactivePower;
  rdfs:domain seas:FeatureOfInterest ;
  rdfs:range seas:ElectricPowerProperty ;
  vs:term_status "testing" ;
  rdfs:isDefinedBy plt:EnergyMeasureOntology.

plt:hasApparentPowerProduction a owl:ObjectProperty , owl:FunctionalProperty ;
  rdfs:label "has apparent power production"@en ;
  rdfs:comment """Links the feature of interest to its apparent power production."""@en ;
  rdfs:subPropertyOf plt:hasPowerProduction , seas:apparentPower;
  rdfs:domain seas:FeatureOfInterest ;
  rdfs:range seas:ElectricPowerProperty ;
  vs:term_status "testing" ;
  rdfs:isDefinedBy plt:EnergyMeasureOntology.


plt:hasPowerConsumption a owl:ObjectProperty , owl:FunctionalProperty ;
  rdfs:label "has power consumption"@en ;
  rdfs:comment """Links the feature of interest to its power consumption."""@en ;
  rdfs:subPropertyOf seas:electricPower ;
  rdfs:domain seas:FeatureOfInterest ;
  rdfs:range seas:ElectricPowerProperty ;
  vs:term_status "testing" ;
  rdfs:isDefinedBy plt:EnergyMeasureOntology.
#######################################
# Energy Load                         #
#######################################
plt:LoadProperty a owl:Class ;
  rdfs:label "Electric  Load Property"@en ;
  rdfs:comment """The class of properties that are quantifiable and have a quantity kind of consumed electric power."""@en ;
  rdfs:subClassOf seas:Property;  
  vs:term_status "testing" ;
  rdfs:isDefinedBy plt:EnergyMeasureOntology .

plt:ElectricEnergyLoadProperty a owl:Class ;
  rdfs:label "Electric Energy Load Property"@en ;
  rdfs:comment """The class of properties that are quantifiable and have a quantity kind of consumed electric power."""@en ;
  rdfs:subClassOf seas:ElectricEnergyProperty,plt:LoadProperty;  
  vs:term_status "testing" ;
  rdfs:isDefinedBy plt:EnergyMeasureOntology .

plt:ElectricEnergyLoadEvaluation a owl:Class ;
  rdfs:label "Electric Energy Load Evaluation"@en ;
  rdfs:comment "The class of evaluation for electric energy load properties"@en ;
  rdfs:subClassOf seas:ElectricEnergyEvaluation;  
  rdfs:subClassOf [ a owl:Restriction ; owl:onProperty seas:evaluationOf ; owl:someValuesFrom plt:ElectricEnergyLoadProperty ] ;
  owl:equivalentClass [ a owl:Restriction ; owl:onProperty seas:evaluationOf ; owl:someValuesFrom plt:ElectricEnergyLoadProperty ] ;
  vs:term_status "testing" ;
  rdfs:isDefinedBy plt:EnergyMeasureOntology .


plt:hasActivePowerReference a owl:ObjectProperty , owl:FunctionalProperty ;
  rdfs:label "has active power reference"@en ;
  rdfs:comment """Links the FeatureOfInterest to its active electric power reference property."""@en ;
  rdfs:subPropertyOf seas:activePower ;
  rdfs:domain seas:FeatureOfInterest ;
  rdfs:range seas:ElectricPowerProperty;
  vs:term_status "testing" ;
  rdfs:isDefinedBy plt:EnergyMeasureOntology  .


plt:hasMinimumActivePower a owl:ObjectProperty , owl:FunctionalProperty ;
  rdfs:label "has minimum active power"@en ;
  rdfs:comment """Links the FeatureOfInterest to its active electric power  property."""@en ;
  rdfs:subPropertyOf seas:activePower ;
  rdfs:domain seas:FeatureOfInterest ;
  rdfs:range seas:ElectricPowerProperty;
  vs:term_status "testing" ;
  rdfs:isDefinedBy plt:EnergyMeasureOntology  .

plt:hasMaximumActivePower a owl:ObjectProperty , owl:FunctionalProperty ;
  rdfs:label "has maximum active power"@en ;
  rdfs:comment """Links the FeatureOfInterest to its active electric power  property."""@en ;
  rdfs:subPropertyOf seas:activePower ;
  rdfs:domain seas:FeatureOfInterest ;
  rdfs:range seas:ElectricPowerProperty;
  vs:term_status "testing" ;
  rdfs:isDefinedBy plt:EnergyMeasureOntology  .
  
plt:hasAverageActivePower a owl:ObjectProperty , owl:FunctionalProperty ;
  rdfs:label "has average active power"@en ;
  rdfs:comment """Links the FeatureOfInterest to its active electric power  property."""@en ;
  rdfs:subPropertyOf seas:activePower ;
  rdfs:domain seas:FeatureOfInterest ;
  rdfs:range seas:ElectricPowerProperty;
  vs:term_status "testing" ;
  rdfs:isDefinedBy plt:EnergyMeasureOntology  .
  
plt:hasStandardDeviationActivePower a owl:ObjectProperty , owl:FunctionalProperty ;
  rdfs:label "has standard deviation active power"@en ;
  rdfs:comment """Links the FeatureOfInterest to its active electric power  property."""@en ;
  rdfs:subPropertyOf seas:activePower ;
  rdfs:domain seas:FeatureOfInterest ;
  rdfs:range seas:ElectricPowerProperty;
  vs:term_status "testing" ;
  rdfs:isDefinedBy plt:EnergyMeasureOntology  .

plt:hasApparentPower a owl:ObjectProperty , owl:FunctionalProperty ;
  rdfs:label "has apparent power"@en ;
  rdfs:comment """Links the FeatureOfInterest to its active electric power  property."""@en ;
  rdfs:subPropertyOf seas:apparentPower ;
  rdfs:domain seas:FeatureOfInterest ;
  rdfs:range seas:ElectricPowerProperty;
  vs:term_status "testing" ;
  rdfs:isDefinedBy plt:EnergyMeasureOntology  .

plt:hasMinimumApparentPower a owl:ObjectProperty , owl:FunctionalProperty ;
  rdfs:label "has minimum apparent power "@en ;
  rdfs:comment """Links the FeatureOfInterest to its active electric power  property."""@en ;
  rdfs:subPropertyOf seas:apparentPower ;
  rdfs:domain seas:FeatureOfInterest ;
  rdfs:range seas:ElectricPowerProperty;
  vs:term_status "testing" ;
  rdfs:isDefinedBy plt:EnergyMeasureOntology  .
  
plt:hasMaximumApparentPower a owl:ObjectProperty , owl:FunctionalProperty ;
  rdfs:label "has maximum apparent power"@en ;
  rdfs:comment """Links the FeatureOfInterest to its apparent electric power  property."""@en ;
  rdfs:subPropertyOf seas:apparentPower ;
  rdfs:domain seas:FeatureOfInterest ;
  rdfs:range seas:ElectricPowerProperty;
  vs:term_status "testing" ;
  rdfs:isDefinedBy plt:EnergyMeasureOntology  .
  
plt:hasAverageApparentPower a owl:ObjectProperty , owl:FunctionalProperty ;
  rdfs:label "has average apparent power"@en ;
  rdfs:comment """Links the FeatureOfInterest to its apparent electric power  property."""@en ;
  rdfs:subPropertyOf seas:apparentPower ;
  rdfs:domain seas:FeatureOfInterest ;
  rdfs:range seas:ElectricPowerProperty;
  vs:term_status "testing" ;
  rdfs:isDefinedBy plt:EnergyMeasureOntology  .
  
plt:hasStandardDeviationApparentPower a owl:ObjectProperty , owl:FunctionalProperty ;
  rdfs:label "has standard deviation apparent power"@en ;
  rdfs:comment """Links the FeatureOfInterest to its apparent electric power property."""@en ;
  rdfs:subPropertyOf seas:apparentPower ;
  rdfs:domain seas:FeatureOfInterest ;
  rdfs:range seas:ElectricPowerProperty;
  vs:term_status "testing" ;
  rdfs:isDefinedBy plt:EnergyMeasureOntology  .
  
plt:hasElectricEnergyLoad a owl:ObjectProperty , owl:FunctionalProperty ;
  rdfs:label "has  electric energy load"@en ;
  rdfs:comment """Links feature of interest to its electric energy load."""@en ;
  rdfs:subPropertyOf plt:hasEnergyLoad;
  rdfs:domain seas:FeatureOfInterest ;
  rdfs:range plt:ElectricEnergyLoadProperty ;
  vs:term_status "testing" ;
  rdfs:isDefinedBy plt:EnergyMeasureOntology  .

plt:hasNominalElectricEnergy a owl:ObjectProperty , owl:FunctionalProperty ;
  rdfs:label "has nominal electric energy"@en ;
  rdfs:comment """Links feature of interest to its nominal electric energy."""@en ;
  rdfs:subPropertyOf seas:electricEnergy ;
  rdfs:domain seas:FeatureOfInterest ;
  rdfs:range seas:ElectricEnergyProperty ;
  vs:term_status "testing" ;
  rdfs:isDefinedBy plt:EnergyMeasureOntology  .

plt:hasElectricEnergyLoadDeviation  a owl:ObjectProperty , owl:FunctionalProperty ;
  rdfs:label "has electric energy load deviation"@en ;
  rdfs:comment """Links the featureOfInterest to its electric energy load deviation."""@en ;
  rdfs:subPropertyOf plt:hasElectricEnergyLoad ;
  rdfs:domain seas:FeatureOfInterest ;
  rdfs:range plt:ElectricEnergyLoadProperty ;
  vs:term_status "testing" ;
  rdfs:isDefinedBy plt:EnergyMeasureOntology  .

plt:HeatingElectricEnergyLoadProperty a owl:Class ;
  rdfs:label "Heating Electric Energy Load Property"@en ;
  rdfs:comment """The class of properties that are quantifiable and have a quantity kind of consumed electric power for heating"""@en ;
  rdfs:subClassOf plt:ElectricEnergyLoadProperty;  
  vs:term_status "testing" ;
  rdfs:isDefinedBy plt:EnergyMeasureOntology .


plt:HeatingElectricEnergyLoadEvaluation a owl:Class ;
  rdfs:label "Heating Electric Energy Load Evaluation"@en ;
  rdfs:comment "The class of evaluation for heating electric energy load properties"@en ;
  rdfs:subClassOf plt:ElectricEnergyLoadEvaluation;
  rdfs:subClassOf [ a owl:Restriction ; owl:onProperty seas:evaluationOf ; owl:someValuesFrom plt:HeatingElectricEnergyLoadProperty ] ;
  owl:equivalentClass [ owl:onProperty seas:evaluationOf ; owl:someValuesFrom plt:HeatingElectricEnergyLoadProperty ] ;
  vs:term_status "testing" ;
  rdfs:isDefinedBy plt:EnergyMeasureOntology .

plt:hasHeatingElectricEnergyLoad a owl:ObjectProperty , owl:FunctionalProperty ;
  rdfs:label "has Heating Electric Energy Load"@en ;
  rdfs:comment """Links the featureOfInterest to its electric energy load for heating."""@en ;
  rdfs:subPropertyOf plt:hasElectricEnergyLoad;
  rdfs:domain seas:FeatureOfInterest ;
  rdfs:range plt:HeatingElectricEnergyLoadProperty ;
  vs:term_status "testing" ;
  rdfs:isDefinedBy plt:EnergyMeasureOntology  .

plt:CoolingElectricEnergyLoadProperty a owl:Class ;
  rdfs:label "Cooling Electric Energy Load Property"@en ;
  rdfs:comment """The class of properties that are quantifiable and have a quantity kind of consumed electric power for cooling"""@en ;
  rdfs:subClassOf plt:ElectricEnergyLoadProperty;  
  vs:term_status "testing" ;
  rdfs:isDefinedBy plt:EnergyMeasureOntology .

plt:CoolingElectricEnergyLoadEvaluation a owl:Class ;
  rdfs:label "Cooling Energy Load Evaluation"@en ;
  rdfs:comment "The class of evaluation for cooling electric energy load properties"@en ;
  rdfs:subClassOf plt:ElectricEnergyLoadEvaluation;  
  rdfs:subClassOf [ a owl:Restriction ; owl:onProperty seas:evaluationOf ; owl:someValuesFrom plt:CoolingElectricEnergyLoadProperty ] ;
  owl:equivalentClass [ owl:onProperty seas:evaluationOf ; owl:someValuesFrom plt:CoolingElectricEnergyLoadProperty ] ;
  vs:term_status "testing" ;
  rdfs:isDefinedBy plt:EnergyMeasureOntology .


plt:hasCoolingElectricEnergyLoad a owl:ObjectProperty , owl:FunctionalProperty ;
  rdfs:label "has Cooling Electric Energy Load"@en ;
  rdfs:comment """Links the feature of interest to its electric energy load."""@en ;
  rdfs:subPropertyOf plt:hasElectricEnergyLoad;
  rdfs:domain seas:FeatureOfInterest ;
  rdfs:range plt:CoolingElectricEnergyLoadProperty ;
  vs:term_status "testing" ;
  rdfs:isDefinedBy plt:EnergyMeasureOntology  .

#######################################
# Forecasting Of Electric Energy Load #
#######################################
plt:ForecastOfElectricEnergyProperty a owl:Class ;
  rdfs:label "Forecast Of Electric Energy  Property"@en ;
  rdfs:comment "The class for forecast of  electric energy  properties"@en ;
  rdfs:subClassOf seas:Forecast; 
  rdfs:subClassOf[ owl:onProperty seas:forecastsProperty ; owl:someValuesFrom seas:ElectricEnergyProperty ] ;
  rdfs:subClassOf[ owl:onProperty pep:madeBy ; owl:someValuesFrom plt:ForecasterOfElectricEnergyProperty ] ;
  vs:term_status "testing" ;
  rdfs:isDefinedBy plt:EnergyMeasureOntology .

plt:ForecasterOfElectricEnergyProperty a owl:Class ;
  rdfs:label "Forecaster Of Energy  Property"@en ;
  rdfs:comment "The class for forecaster of energy  properties"@en ;
  rdfs:subClassOf seas:Forecaster; 
  rdfs:subClassOf[ owl:onProperty seas:forecastsProperty ; owl:someValuesFrom seas:ElectricEnergyProperty ] ;
  rdfs:subClassOf[ owl:onProperty pep:implements ; owl:someValuesFrom plt:ForecastingOfElectricEnergyProperty ] ;
  vs:term_status "testing" ;
  rdfs:isDefinedBy plt:EnergyMeasureOntology .

plt:ForecastingOfElectricEnergyProperty a owl:Class ;
  rdfs:label "Forecasting Of Electric Energy  Property"@en ;
  rdfs:comment "The class for forecasting of electric energy  properties"@en ;
  rdfs:subClassOf seas:Forecasting; 
  rdfs:subClassOf[ owl:onProperty seas:forecastsProperty ; owl:someValuesFrom seas:ElectricEnergyProperty ] ;
  vs:term_status "testing" ;
  rdfs:isDefinedBy plt:EnergyMeasureOntology .

plt:hasForecastOfElectricEnergyProperty a owl:ObjectProperty , owl:FunctionalProperty ;
  rdfs:label "has forecast of electric energy  property"@en ;
  rdfs:comment """Links Feature Of Interest with  its forecast of electric energy  property."""@en ;
  rdfs:subPropertyOf plt:hasForecastOfProperty;
  rdfs:domain saref:FeatureOfInterest ;
  rdfs:range plt:ForecastOfElectricEnergyProperty ;
  vs:term_status "testing" ;
  rdfs:isDefinedBy plt:EnergyMeasureOntology .


plt:ForecastOfElectricEnergyLoadProperty a owl:Class ;
  rdfs:label "Forecast Of Electric Energy Load Property"@en ;
  rdfs:comment "The class for forecast of  electric energy load properties"@en ;
  rdfs:subClassOf plt:ForecastOfElectricEnergyProperty ; 
  rdfs:subClassOf[ owl:onProperty seas:forecastsProperty ; owl:someValuesFrom plt:ElectricEnergyLoadProperty ] ;
  rdfs:subClassOf[ owl:onProperty pep:madeBy ; owl:someValuesFrom plt:ForecasterOfElectricEnergyLoadProperty ] ;
  vs:term_status "testing" ;
  rdfs:isDefinedBy plt:EnergyMeasureOntology .

plt:ForecasterOfElectricEnergyLoadProperty a owl:Class ;
  rdfs:label "Forecaster Of Energy Load Property"@en ;
  rdfs:comment "The class for forecaster of energy load properties"@en ;
  rdfs:subClassOf plt:ForecasterOfElectricEnergyProperty ; 
  rdfs:subClassOf[ owl:onProperty seas:forecastsProperty ; owl:someValuesFrom plt:ElectricEnergyLoadProperty ] ;
  rdfs:subClassOf[ owl:onProperty pep:implements ; owl:someValuesFrom plt:ForecastingOfElectricEnergyLoadProperty ] ;
    rdfs:subClassOf[ owl:onProperty pep:made ; owl:someValuesFrom plt:ForecastOfElectricEnergyLoadProperty ] ;

  vs:term_status "testing" ;
  rdfs:isDefinedBy plt:EnergyMeasureOntology .

plt:ForecastingOfElectricEnergyLoadProperty a owl:Class ;
  rdfs:label "Forecasting Of Electric Energy Load Property"@en ;
  rdfs:comment "The class for forecasting of electric energy load properties"@en ;
  rdfs:subClassOf plt:ForecastingOfElectricEnergyProperty ; 
  rdfs:subClassOf[ owl:onProperty seas:forecastsProperty ; owl:someValuesFrom plt:ElectricEnergyLoadProperty ] ;
  vs:term_status "testing" ;
  rdfs:isDefinedBy plt:EnergyMeasureOntology .

plt:hasForecastOfElectricEnergyLoadProperty a owl:ObjectProperty , owl:FunctionalProperty ;
  rdfs:label "has forecast of electric energy load property"@en ;
  rdfs:comment """Links Feature Of Interest with  its forecast of electric energy load property."""@en ;
  rdfs:subPropertyOf plt:hasForecastOfElectricEnergyProperty;
  rdfs:domain saref:FeatureOfInterest ;
  rdfs:range plt:ForecastOfElectricEnergyLoadProperty ;
  vs:term_status "testing" ;
  rdfs:isDefinedBy plt:EnergyMeasureOntology .

plt:nominalElectricalCurrent a owl:ObjectProperty , owl:FunctionalProperty ;
  rdfs:label "nominal electrical current"@en ;
  rdfs:comment """Links the feature of interest to its nominal electrical current."""@en ;
  rdfs:subPropertyOf seas:electricalCurrent;
  rdfs:domain seas:FeatureOfInterest ;
  rdfs:range seas:CurrentProperty ;
  vs:term_status "testing" ;
  rdfs:isDefinedBy plt:EnergyMeasureOntology  .

plt:hasOutputCurrent a owl:ObjectProperty , owl:FunctionalProperty ;
  rdfs:label "has output current"@en ;
  rdfs:comment """Links the feature of interest to its output current."""@en ;
  rdfs:subPropertyOf seas:electricalCurrent;
  rdfs:domain seas:FeatureOfInterest ;
  rdfs:range seas:CurrentProperty ;
  vs:term_status "testing" ;
  rdfs:isDefinedBy plt:EnergyMeasureOntology  .

plt:hasInputCurrent a owl:ObjectProperty , owl:FunctionalProperty ;
  rdfs:label "has input current"@en ;
  rdfs:comment """Links the feature of interest to its input current."""@en ;
  rdfs:subPropertyOf seas:electricalCurrent;
  rdfs:domain seas:FeatureOfInterest ;
  rdfs:range seas:CurrentProperty ;
  vs:term_status "testing" ;
  rdfs:isDefinedBy plt:EnergyMeasureOntology  .

plt:hasAverageRCurrent a owl:ObjectProperty , owl:FunctionalProperty ;
  rdfs:label "has average r current"@en ;
  rdfs:comment """Links a three-phase connection point to the average current in its R wire."""@en ;
  rdfs:subPropertyOf seas:rCurrent;
  rdfs:domain seas:ThreePhaseConnectionPoint ;
  rdfs:range seas:CurrentProperty ;
  vs:term_status "testing" ;
  rdfs:isDefinedBy plt:EnergyMeasureOntology  .

plt:hasAverageSCurrent a owl:ObjectProperty , owl:FunctionalProperty ;
  rdfs:label "has average s current"@en ;
  rdfs:comment """Links a three-phase connection point to the average current in its S wire."""@en ;
  rdfs:subPropertyOf seas:sCurrent;
  rdfs:domain seas:ThreePhaseConnectionPoint ;
  rdfs:range seas:CurrentProperty ;
  vs:term_status "testing" ;
  rdfs:isDefinedBy plt:EnergyMeasureOntology  .

plt:hasAverageTCurrent a owl:ObjectProperty , owl:FunctionalProperty ;
  rdfs:label "has average t current"@en ;
  rdfs:comment """Links a three-phase connection point to the average current in its T wire."""@en ;
  rdfs:subPropertyOf seas:tCurrent;
  rdfs:domain seas:ThreePhaseConnectionPoint ;
  rdfs:range seas:CurrentProperty ;
  vs:term_status "testing" ;
  rdfs:isDefinedBy plt:EnergyMeasureOntology  .


#######################################

# electricPowerGenerationCapacity #

#######################################
plt:ElectricPowerGenerationCapacityProperty  a owl:Class ;
  rdfs:label "Electric Power Generation Capacity Property"@en ;
  rdfs:comment """The class of properties that are quantifiable and have a quantity electric power generation capacity"""@en ;
  rdfs:subClassOf seas:ElectricPowerProperty;  
vs:term_status "testing" ;
  rdfs:isDefinedBy plt:EnergyMeasureOntology  .

plt:hasElectricPowerGenerationCapacity a owl:ObjectProperty , owl:FunctionalProperty ;
  rdfs:label "electric power generation capacity"@en ;
  rdfs:comment """Links some electric power system, such as Thermal Storage System to its electric power generation capacityt property."""@en ;
  rdfs:subPropertyOf seas:hasProperty;
  rdfs:domain seas:ElectricPowerSystem ;
  rdfs:range plt:ElectricPowerGenerationCapacityProperty ;
  vs:term_status "testing" ;
  rdfs:isDefinedBy plt:EnergyMeasureOntology  .

#######################################
#  Voltage                            #
#######################################
plt:hasLowVoltageLimit a owl:ObjectProperty , owl:FunctionalProperty ;
  rdfs:label "has low voltage limit"@en ;
  rdfs:comment """Links the feature of interest to its low voltage limit."""@en ;
  rdfs:subPropertyOf seas:voltage;
  rdfs:domain seas:FeatureOfInterest ;
  rdfs:range seas:VoltageProperty ;
  vs:term_status "testing" ;
  rdfs:isDefinedBy plt:EnergyMeasureOntology  .

plt:hasHighVoltageLimit a owl:ObjectProperty , owl:FunctionalProperty ;
  rdfs:label "has high voltage limit"@en ;
  rdfs:comment """Links the feature of interest to its high voltage limit."""@en ;
  rdfs:subPropertyOf seas:voltage;
  rdfs:domain seas:FeatureOfInterest ;
  rdfs:range seas:VoltageProperty ;
  vs:term_status "testing" ;
  rdfs:isDefinedBy plt:EnergyMeasureOntology  .


plt:hasNominalVoltage  a owl:ObjectProperty , owl:FunctionalProperty ;
  rdfs:label "has nominal voltage"@en ;
  rdfs:comment """Links the feature of interest to its nominal voltage."""@en ;
  rdfs:subPropertyOf seas:voltage;
  rdfs:domain seas:FeatureOfInterest ;
  rdfs:range seas:VoltageProperty ;
  vs:term_status "testing" ;
  rdfs:isDefinedBy plt:EnergyMeasureOntology  .

plt:hasOutputVoltage  a owl:ObjectProperty , owl:FunctionalProperty ;
  rdfs:label "has output voltage"@en ;
  rdfs:comment """Links the feature of interest to its output voltage."""@en ;
  rdfs:subPropertyOf seas:voltage;
  rdfs:domain seas:FeatureOfInterest ;
  rdfs:range seas:VoltageProperty ;
  vs:term_status "testing" ;
  rdfs:isDefinedBy plt:EnergyMeasureOntology  .

plt:hasInputVoltage  a owl:ObjectProperty , owl:FunctionalProperty ;
  rdfs:label "has input voltage"@en ;
  rdfs:comment """Links the feature of interest to its input voltage."""@en ;
  rdfs:subPropertyOf seas:voltage;
  rdfs:domain seas:FeatureOfInterest ;
  rdfs:range seas:VoltageProperty ;
  vs:term_status "testing" ;
  rdfs:isDefinedBy plt:EnergyMeasureOntology  .

plt:hasAverageRNVoltage a owl:ObjectProperty , owl:FunctionalProperty ;
  rdfs:label "has average voltage"@en ;
  rdfs:comment """LLinks a three-phase power bus or a three-phase connection point to the average voltage between its R and its N wires."""@en ;
  rdfs:subPropertyOf seas:RNVoltage;
  rdfs:domain seas:FeatureOfInterest ;
  rdfs:range seas:VoltageProperty ;
  vs:term_status "testing" ;
  rdfs:isDefinedBy plt:EnergyMeasureOntology  .

plt:hasAverageSNVoltage a owl:ObjectProperty , owl:FunctionalProperty ;
  rdfs:label "has average voltage"@en ;
  rdfs:comment """Links a three-phase power bus or a three-phase connection point to the average voltage between its S and its N wires."""@en ;
  rdfs:subPropertyOf seas:SNVoltage;
  rdfs:domain seas:FeatureOfInterest ;
  rdfs:range seas:VoltageProperty ;
  vs:term_status "testing" ;
  rdfs:isDefinedBy plt:EnergyMeasureOntology  .

plt:hasAverageTNVoltage a owl:ObjectProperty , owl:FunctionalProperty ;
  rdfs:label "has average voltage"@en ;
  rdfs:comment """Links a three-phase power bus or a three-phase connection point to the average voltage between its T and its N wires."""@en ;
  rdfs:subPropertyOf seas:TNVoltage;
  rdfs:domain seas:FeatureOfInterest ;
  rdfs:range seas:VoltageProperty ;
  vs:term_status "testing" ;
  rdfs:isDefinedBy plt:EnergyMeasureOntology  .
#######################################
# active Power                        #
#######################################
plt:hasCapacityActivePower a owl:ObjectProperty , owl:FunctionalProperty ;
  rdfs:label "has capacity active power"@en ;
  rdfs:comment """Links the FeatureOfInterest to its capacity active power property."""@en ;
  rdfs:subPropertyOf seas:activePower  ;
  rdfs:domain seas:FeatureOfInterest ;
  rdfs:range seas:ElectricPowerProperty;
  vs:term_status "testing" ;
  rdfs:isDefinedBy plt:EnergyMeasureOntology  .

plt:hasMaximalCapacityActivePower a owl:ObjectProperty , owl:FunctionalProperty ;
  rdfs:label "has maximal capacity active power"@en ;
  rdfs:comment """Links the FeatureOfInterest to its maximal capacity active power property."""@en ;
  rdfs:subPropertyOf seas:activePower          ;
  rdfs:domain seas:FeatureOfInterest ;
  rdfs:range seas:ElectricPowerProperty;
  vs:term_status "testing" ;
  rdfs:isDefinedBy plt:EnergyMeasureOntology  .

plt:hasMinimalCapacityActivePower a owl:ObjectProperty , owl:FunctionalProperty ;
  rdfs:label "has minimal capacity active power"@en ;
  rdfs:comment """Links the FeatureOfInterest to its minimal capacity active power property."""@en ;
  rdfs:subPropertyOf seas:activePower ;
  rdfs:domain seas:FeatureOfInterest ;
  rdfs:range seas:ElectricPowerProperty;
  vs:term_status "testing" ;
  rdfs:isDefinedBy plt:EnergyMeasureOntology  .

plt:hasDefaultCapacityActivePower a owl:ObjectProperty , owl:FunctionalProperty ;
  rdfs:label "has default capacity active power"@en ;
  rdfs:comment """Links the FeatureOfInterest to its default capacity active power property."""@en ;
  rdfs:subPropertyOf seas:activePower ;
  rdfs:domain seas:FeatureOfInterest ;
  rdfs:range seas:ElectricPowerProperty;
  vs:term_status "testing" ;
  rdfs:isDefinedBy plt:EnergyMeasureOntology .

plt:hasNetInterchangeActivePower a owl:ObjectProperty , owl:FunctionalProperty ;
  rdfs:label "has net interchange active power"@en ;
  rdfs:comment """Links the FeatureOfInterest to its net interchange active power property."""@en ;
  rdfs:subPropertyOf seas:activePower ;
  rdfs:domain seas:FeatureOfInterest ;
  rdfs:range seas:ElectricPowerProperty;
  vs:term_status "testing" ;
  rdfs:isDefinedBy plt:EnergyMeasureOntology .


plt:hasNetInterchangeToleranceActivePower a owl:ObjectProperty , owl:FunctionalProperty ;
  rdfs:label "has net interchange tolerance active power"@en ;
  rdfs:comment """Links the FeatureOfInterest to its net interchange tolerance active power property."""@en ;
  rdfs:subPropertyOf seas:activePower ;
  rdfs:domain seas:FeatureOfInterest ;
  rdfs:range seas:ElectricPowerProperty;
  vs:term_status "testing" ;
  rdfs:isDefinedBy plt:EnergyMeasureOntology .

#######################################
# thermal Load                       #
#######################################
plt:ThermalEnergyProperty a owl:Class ;
  rdfs:label "Thermal Energy Property"@en ;
  rdfs:comment "The class of properties that are quantifiable and have a quantity kind of thermmal power."@en ;
  rdfs:subClassOf plt:EnergyProperty ;
  vs:term_status "testing" ;
  rdfs:isDefinedBy plt:EnergyMeasureOntology .

plt:ThermalEnergyLoadProperty a owl:Class ;
  rdfs:label "Thermal Energy Load Property"@en ;
  skos:altLabel "Thermal Power";
  rdfs:comment """The class of properties that are quantifiable and have a quantity kind of consumed thermmal power"""@en ;
  rdfs:subClassOf plt:ThermalEnergyProperty ,plt:LoadProperty;
  vs:term_status "testing" ;
  rdfs:isDefinedBy plt:EnergyMeasureOntology .

plt:ThermalEnergyLoadEvaluation a owl:Class ;
  rdfs:label "Thermal Energy Load Evaluation"@en ;
  rdfs:comment "The class of evaluation for thermmal energy load properties"@en ;
  rdfs:subClassOf seas:Evaluation;  
  rdfs:subClassOf [ a owl:Restriction ; owl:onProperty seas:evaluationOf ; owl:someValuesFrom plt:ThermalEnergyLoadProperty ] ;
  owl:equivalentClass [ owl:onProperty seas:evaluationOf ; owl:someValuesFrom plt:ThermalEnergyLoadProperty ] ;
  vs:term_status "testing" ;
  rdfs:isDefinedBy plt:EnergyMeasureOntology .

plt:hasEnergyLoad a owl:ObjectProperty , owl:FunctionalProperty ;
  rdfs:label "has  energy load"@en ;
  rdfs:comment """Links Feature Of Interest to its  energy load."""@en ;
  rdfs:subPropertyOf plt:hasEnergy;
  rdfs:domain seas:FeatureOfInterest ;
  rdfs:range plt:ThermalEnergyLoadProperty ;
  vs:term_status "testing" ;
  rdfs:isDefinedBy plt:EnergyMeasureOntology.

plt:hasThermalEnergyLoad a owl:ObjectProperty , owl:FunctionalProperty ;
  rdfs:label "has thermal energy load"@en ;
  rdfs:comment """Links Feature Of Interest to its thermmal energy load."""@en ;
  rdfs:subPropertyOf plt:hasEnergyLoad;
  rdfs:domain seas:FeatureOfInterest ;
  rdfs:range plt:ThermalEnergyLoadProperty ;
  vs:term_status "testing" ;
  rdfs:isDefinedBy plt:EnergyMeasureOntology.

plt:hasNominalThermalPower a owl:ObjectProperty , owl:FunctionalProperty ;
  rdfs:label "has thermal energy load"@en ;
  rdfs:comment """Links Feature Of Interest to its nominal thermmal energy power."""@en ;
  rdfs:subPropertyOf plt:hasNominalPower ;
  rdfs:domain seas:FeatureOfInterest ;
  rdfs:range plt:ThermalEnergyLoadProperty ;
  vs:term_status "testing" ;
  rdfs:isDefinedBy plt:EnergyMeasureOntology.

plt:hasNetInterchangeActivePower a owl:ObjectProperty , owl:FunctionalProperty ;
  rdfs:label "has net interchange active power"@en ;
  rdfs:comment """Links the FeatureOfInterest to its net interchange active power property."""@en ;
  rdfs:subPropertyOf seas:activePower  ;
  rdfs:domain seas:FeatureOfInterest ;
  rdfs:range cim:ActivePower;
  vs:term_status "testing" ;
  rdfs:isDefinedBy plt:EnergyMeasureOntology .

plt:hasNetInterchangeToleranceActivePower a owl:ObjectProperty , owl:FunctionalProperty ;
  rdfs:label "has net interchange tolerance active power"@en ;
  rdfs:comment """Links the FeatureOfInterest to its net interchange tolerance active power property."""@en ;
  rdfs:subPropertyOf seas:activePower  ;
  rdfs:domain seas:FeatureOfInterest ;
  rdfs:range cim:ActivePower;
  vs:term_status "testing" ;
  rdfs:isDefinedBy plt:EnergyMeasureOntology  .
#######################################
# electrical Loss                     #
####################################### 
plt:ElectricalLossProperty a owl:Class ;
  rdfs:label "Electrical Loss Property"@en ;
  rdfs:comment """The class of properties that are quantifiable and have a quantity kind of electrical loss"""@en ;
  rdfs:subClassOf seas:ElectricEnergyProperty;  
  vs:term_status "testing" ;
  rdfs:isDefinedBy plt:EnergyMeasureOntology .


plt:ElectricalLossEvaluation a owl:Class ;
  rdfs:label "Electrical Loss Evaluation"@en ;
  rdfs:comment "The class of evaluation for electrical loss properties"@en ;
  rdfs:subClassOf seas:ElectricEnergyEvaluation;  
  rdfs:subClassOf [ a owl:Restriction ; owl:onProperty seas:evaluationOf ; owl:someValuesFrom plt:ElectricalLossProperty ] ;
  owl:equivalentClass [ owl:onProperty seas:evaluationOf ; owl:someValuesFrom plt:ElectricalLossProperty ] ;
  vs:term_status "testing" ;
  rdfs:isDefinedBy plt:EnergyMeasureOntology .


plt:hasElectricalLoss a owl:ObjectProperty , owl:FunctionalProperty ;
  rdfs:label "has electrical loss"@en ;
  rdfs:comment """Links the feature of interest,such as electric power transformer, to its electrical loss."""@en ;
  rdfs:subPropertyOf seas:electricEnergy;
  rdfs:domain seas:FeatureOfInterest ;
  rdfs:range seas:electricEnergy ;
  vs:term_status "testing" ;
  rdfs:isDefinedBy plt:EnergyMeasureOntology .

#######################################
# physical power                     #
####################################### 
plt:PhysicalPowerProperty a owl:Class ;
  rdfs:label "Physical Power Property"@en ;
  rdfs:comment """The class of properties that are quantifiable and have a quantity kind of physical power"""@en ;
  rdfs:subClassOf seas:ElectricEnergyProperty;  
  vs:term_status "testing" ;
  rdfs:isDefinedBy plt:EnergyMeasureOntology .


plt:PhysicalPowerEvaluation a owl:Class ;
  rdfs:label "Physical Power Evaluation"@en ;
  rdfs:comment "The class of evaluation for physical power properties"@en ;
  rdfs:subClassOf seas:ElectricEnergyEvaluation;  
  rdfs:subClassOf [ a owl:Restriction ; owl:onProperty seas:evaluationOf ; owl:someValuesFrom plt:PhysicalPowerProperty ] ;
  owl:equivalentClass [ owl:onProperty seas:evaluationOf ; owl:someValuesFrom plt:PhysicalPowerProperty ] ;
  vs:term_status "testing" ;
  rdfs:isDefinedBy plt:EnergyMeasureOntology .


plt:hasPhysicalPower a owl:ObjectProperty , owl:FunctionalProperty ;
  rdfs:label "has physical power"@en ;
  rdfs:comment """Links the feature of interest,such as cable, to its physical power."""@en ;
  rdfs:subPropertyOf seas:hasProperty;
  rdfs:domain seas:FeatureOfInterest ;
  rdfs:range plt:PhysicalPowerProperty ;
  vs:term_status "testing" ;
  rdfs:isDefinedBy plt:EnergyMeasureOntology .

plt:hasMinimumPhysicalPower a owl:ObjectProperty , owl:FunctionalProperty ;
  rdfs:label "has minimum physical power"@en ;
  rdfs:comment """Links the feature of interest to its minimum physical power."""@en ;
  rdfs:subPropertyOf plt:hasPhysicalPower ;
  rdfs:domain seas:FeatureOfInterest ;
  rdfs:range plt:PhysicalPowerProperty ;
  vs:term_status "testing" ;
  rdfs:isDefinedBy plt:EnergyMeasureOntology .

plt:hasMaximumPhysicalPower a owl:ObjectProperty , owl:FunctionalProperty ;
  rdfs:label "has maximum physical power"@en ;
  rdfs:comment """Links the feature of interest to its maximum physical power."""@en ;
  rdfs:subPropertyOf plt:hasPhysicalPower ;
  rdfs:domain seas:FeatureOfInterest ;
  rdfs:range plt:PhysicalPowerProperty ;
  vs:term_status "testing" ;
  rdfs:isDefinedBy plt:EnergyMeasureOntology .

plt:hasAveragePhysicalPower a owl:ObjectProperty , owl:FunctionalProperty ;
  rdfs:label "has  average physical power"@en ;
  rdfs:comment """Links the feature of interest to its average physical power."""@en ;
  rdfs:subPropertyOf plt:hasPhysicalPower ;
  rdfs:domain seas:FeatureOfInterest ;
  rdfs:range plt:PhysicalPowerProperty ;
  vs:term_status "testing" ;
  rdfs:isDefinedBy plt:EnergyMeasureOntology .

plt:hasStandardDeviationPhysicalPower a owl:ObjectProperty , owl:FunctionalProperty ;
  rdfs:label "has standard deviation physical power"@en ;
  rdfs:comment """Links the feature of interest to its standard deviation physical power."""@en ;
  rdfs:subPropertyOf plt:hasPhysicalPower ;
  rdfs:domain seas:FeatureOfInterest ;
  rdfs:range plt:PhysicalPowerProperty ;
  vs:term_status "testing" ;
  rdfs:isDefinedBy plt:EnergyMeasureOntology .
#######################################
# power consumption pattern           #
####################################### 
plt:PowerConsumptionPatternProperty a owl:Class ;
  rdfs:label "Power Consumption Pattern Property"@en ;
  rdfs:comment """The class of properties that are quantifiable and have a quantity kind of power consumption pattern"""@en ;
  rdfs:subClassOf seas:Property;  
  vs:term_status "testing" ;
  rdfs:isDefinedBy plt:EnergyMeasureOntology .


plt:PowerConsumptionPatternEvaluation a owl:Class ;
  rdfs:label "Power Consumption Pattern Evaluation"@en ;
  rdfs:comment "The class of evaluation for power consumption pattern properties"@en ;
  rdfs:subClassOf seas:Evaluation;  
  rdfs:subClassOf [ a owl:Restriction ; owl:onProperty seas:evaluationOf ; owl:someValuesFrom plt:PowerConsumptionPatternProperty ] ;
  owl:equivalentClass [ owl:onProperty seas:evaluationOf ; owl:someValuesFrom plt:PowerConsumptionPatternProperty ] ;
  vs:term_status "testing" ;
  rdfs:isDefinedBy plt:EnergyMeasureOntology .


plt:hasPowerConsumptionPattern a owl:ObjectProperty , owl:FunctionalProperty ;
  rdfs:label "has power consumption pattern"@en ;
  rdfs:comment """Links the feature of interest,such as electric power transformer, to its power consumption pattern."""@en ;
  rdfs:subPropertyOf seas:hasProperty ;
  rdfs:domain seas:FeatureOfInterest ;
  rdfs:range plt:PowerConsumptionPatternProperty ;
  vs:term_status "testing" ;
  rdfs:isDefinedBy plt:EnergyMeasureOntology .

#######################################
# solar energy                        #
####################################### 
plt:SolarEnergyProperty a owl:Class ;
  rdfs:label "Solar Energy Property"@en ;
  rdfs:comment """The class of properties that are quantifiable and have a quantity kind of solar energy"""@en ;
  rdfs:subClassOf plt:EnergyProperty;  
  vs:term_status "testing" ;
  rdfs:isDefinedBy plt:EnergyMeasureOntology .


plt:SolarEnergyEvaluation a owl:Class ;
  rdfs:label "Solar Energy Evaluation"@en ;
  rdfs:comment "The class of evaluation for solar energy properties"@en ;
  rdfs:subClassOf plt:EnergyEvaluation;  
  rdfs:subClassOf [ a owl:Restriction ; owl:onProperty seas:evaluationOf ; owl:someValuesFrom plt:SolarEnergyProperty ] ;
  owl:equivalentClass [ owl:onProperty seas:evaluationOf ; owl:someValuesFrom plt:SolarEnergyProperty ] ;
  vs:term_status "testing" ;
  rdfs:isDefinedBy plt:EnergyMeasureOntology .


plt:hasSolarEnergy a owl:ObjectProperty , owl:FunctionalProperty ;
  rdfs:label "has solar energy"@en ;
  rdfs:comment """Links the feature of interest,such as solar storage system, to its solar energy."""@en ;
  rdfs:subPropertyOf plt:hasEnergy;
  rdfs:domain seas:FeatureOfInterest ;
  rdfs:range plt:SolarEnergyProperty ;
  vs:term_status "testing" ;
  rdfs:isDefinedBy plt:EnergyMeasureOntology .

#######################################
# power factor                        #
####################################### 

plt:PowerFactorProperty a owl:Class ;
  rdfs:label "Power Factor Property"@en ;
  skos:altLabel "Cos phi"@en ;
  rdfs:comment """electrical power system is defined as the ratio of the real power absorbed by the load to the apparent power flowing in the circuit, and is a dimensionless number in the closed interval of ‚àí1 to 1. source: wikipedia"""@en ;
  rdfs:subClassOf seas:Property;  
  vs:term_status "testing" ;
  rdfs:isDefinedBy plt:EnergyMeasureOntology .

plt:PowerFactorEvaluation a owl:Class ;
  rdfs:label "Power Factor Evaluation"@en ;
  rdfs:comment "The class of evaluation for power factor properties"@en ;
  rdfs:subClassOf seas:Evaluation;  
  rdfs:subClassOf [ a owl:Restriction ; owl:onProperty seas:evaluationOf ; owl:someValuesFrom plt:PowerFactorProperty ] ;
  owl:equivalentClass [ owl:onProperty seas:evaluationOf ; owl:someValuesFrom plt:PowerFactorProperty ] ;
  vs:term_status "testing" ;
  rdfs:isDefinedBy plt:EnergyMeasureOntology .

plt:hasPowerFactor a owl:ObjectProperty , owl:FunctionalProperty ;
  rdfs:label "has power factor"@en ;
  rdfs:comment """Links the feature of interest to its power factor."""@en ;
  rdfs:subPropertyOf seas:electricPower;
  owl:equivalentProperty seas:powerFactor ;
  rdfs:domain seas:FeatureOfInterest ;
  rdfs:range plt:PowerFactorProperty ;
  vs:term_status "testing" ;
  rdfs:isDefinedBy plt:EnergyMeasureOntology .

plt:hasMinimumPowerFactor a owl:ObjectProperty , owl:FunctionalProperty ;
  rdfs:label "has power minimum factor"@en ;
  rdfs:comment """Links the feature of interest to its power factor."""@en ;
  rdfs:subPropertyOf plt:hasPowerFactor ;
  rdfs:domain seas:FeatureOfInterest ;
  rdfs:range plt:PowerFactorProperty ;
  vs:term_status "testing" ;
  rdfs:isDefinedBy plt:EnergyMeasureOntology .

plt:hasMaximumPowerFactor a owl:ObjectProperty , owl:FunctionalProperty ;
  rdfs:label "has power maximum factor"@en ;
  rdfs:comment """Links the feature of interest to its power factor."""@en ;
  rdfs:subPropertyOf plt:hasPowerFactor ;
  rdfs:domain seas:FeatureOfInterest ;
  rdfs:range plt:PowerFactorProperty ;
  vs:term_status "testing" ;
  rdfs:isDefinedBy plt:EnergyMeasureOntology .

plt:hasAveragePowerFactor a owl:ObjectProperty , owl:FunctionalProperty ;
  rdfs:label "has power average factor"@en ;
  rdfs:comment """Links the feature of interest to its power factor."""@en ;
  rdfs:subPropertyOf plt:hasPowerFactor ;
  rdfs:domain seas:FeatureOfInterest ;
  rdfs:range plt:PowerFactorProperty ;
  vs:term_status "testing" ;
  rdfs:isDefinedBy plt:EnergyMeasureOntology .

plt:hasStandardDeviationPowerFactor a owl:ObjectProperty , owl:FunctionalProperty ;
  rdfs:label "has power satandard deviation factor"@en ;
  rdfs:comment """Links the feature of interest to its power factor."""@en ;
  rdfs:subPropertyOf plt:hasPowerFactor ;
  rdfs:domain seas:FeatureOfInterest ;
  rdfs:range plt:PowerFactorProperty ;
  vs:term_status "testing" ;
  rdfs:isDefinedBy plt:EnergyMeasureOntology .
#######################################
#   StatusPowerCurve          #
#######################################

plt:StatusPowerCurveProperty a owl:Class ;
  rdfs:label "Status Power Curve Property"@en ;
  rdfs:comment """The class of properties that are quantifiable and have a quantity status power curve"""@en ;
  rdfs:subClassOf seas:Property;  
  vs:term_status "testing" ;
  rdfs:isDefinedBy plt:EnergyMeasureOntology .


plt:StatusPowerCurveEvaluation a owl:Class ;
  rdfs:label "Status Power Curve Evaluation"@en ;
  rdfs:comment "The class of evaluation for rotational status power curve"@en ;
  rdfs:subClassOf seas:Evaluation;  
  rdfs:subClassOf [ a owl:Restriction ; owl:onProperty seas:evaluationOf ; owl:someValuesFrom plt:StatusPowerCurveProperty ] ;
  owl:equivalentClass [ owl:onProperty seas:evaluationOf ; owl:someValuesFrom plt:StatusPowerCurveProperty ] ;
  vs:term_status "testing" ;
  rdfs:isDefinedBy plt:EnergyMeasureOntology .

plt:hasStatusPowerCurve a owl:ObjectProperty , owl:FunctionalProperty ;
  rdfs:label "has  status power curve "@en ;
  rdfs:comment """Link the electric power system to its  status power curve."""@en ;
  rdfs:subPropertyOf seas:hasProperty;
  rdfs:domain seas:ElectricPowerSystem ;
  rdfs:range seas:StatusPowerCurveProperty;
  vs:term_status "testing" ;
  rdfs:isDefinedBy plt:EnergyMeasureOntology.


plt:hasMinimumStatusPowerCurve a owl:ObjectProperty , owl:FunctionalProperty ;
  rdfs:label "has minimum status power curve "@en ;
  rdfs:comment """Link the electric power system to its  status power curve."""@en ;
  rdfs:subPropertyOf plt:hasStatusPowerCurve ;
  rdfs:domain seas:ElectricPowerSystem ;
  rdfs:range seas:StatusPowerCurveProperty;
  vs:term_status "testing" ;
  rdfs:isDefinedBy plt:EnergyMeasureOntology.


plt:hasMaximumStatusPowerCurve a owl:ObjectProperty , owl:FunctionalProperty ;
  rdfs:label "has maximum status power curve "@en ;
  rdfs:comment """Link the electric power system to its  status power curve."""@en ;
  rdfs:subPropertyOf plt:hasStatusPowerCurve ;
  rdfs:domain seas:ElectricPowerSystem ;
  rdfs:range seas:StatusPowerCurveProperty;
  vs:term_status "testing" ;
  rdfs:isDefinedBy plt:EnergyMeasureOntology.

plt:hasAverageStatusPowerCurve a owl:ObjectProperty , owl:FunctionalProperty ;
  rdfs:label "has average status power curve "@en ;
  rdfs:comment """Link the electric power system to its  status power curve."""@en ;
  rdfs:subPropertyOf plt:hasStatusPowerCurve ;
  rdfs:domain seas:ElectricPowerSystem ;
  rdfs:range seas:StatusPowerCurveProperty;
  vs:term_status "testing" ;
  rdfs:isDefinedBy plt:EnergyMeasureOntology.

plt:hasStandardDeviationStatusPowerCurve a owl:ObjectProperty , owl:FunctionalProperty ;
  rdfs:label "has standard deviation status power curve "@en ;
  rdfs:comment """Link the electric power system to its  status power curve."""@en ;
  rdfs:subPropertyOf plt:hasStatusPowerCurve ;
  rdfs:domain seas:ElectricPowerSystem ;
  rdfs:range seas:StatusPowerCurveProperty;
  vs:term_status "testing" ;
  rdfs:isDefinedBy plt:EnergyMeasureOntology.
#######################################
#   Frequency          #
#######################################
plt:hasFrequencyGridSide a owl:ObjectProperty , owl:FunctionalProperty ;
  rdfs:label "has frequency grid side "@en ;
  rdfs:comment """Link the electric power system to its frequency grid side."""@en ;
  rdfs:subPropertyOf plt:hasStatusPowerCurve ;
  rdfs:domain seas:ElectricPowerSystem ;
  rdfs:range seas:FrequencyProperty;
  vs:term_status "testing" ;
  rdfs:isDefinedBy plt:EnergyMeasureOntology.
#######################################
#   reused concepts                   #
#######################################

seas:ElectricPowerProperty a owl:Class.
seas:ElectricPowerEvaluation a owl:Class.

seas:ElectricEnergyProperty a owl:Class.
seas:ElectricEnergyEvaluation a owl:Class.

seas:FrequencyProperty a owl:Class.
seas:FrequencyEvaluation a owl:Class.

seas:CurrentProperty a owl:Class.
seas:CurrentEvaluation a owl:Class.


seas:VoltageProperty a owl:Class.
seas:VoltageEvalution a owl:Class.


seas:EfficencyProperty a owl:Class.

seas:EfficencyEvalution a owl:Class.

cim:ActivePower a owl:Class.

cim:ReactivePower a owl:Class.

saref:Energy a owl:Class.

seas:ConsumptionProperty a owl:Class.

seas:ElectricEnergyProperty a owl:Class.

seas:FeatureOfInterest a owl:Class.

seas:Evaluation a owl:Class.

seas:Property a owl:Class.

saref:Power a owl:Class.

seas:Forecast a owl:Class.
#######################################
#   reused relations                   #
#######################################

seas:reactivePower a owl:ObjectProperty.

seas:activePower a owl:ObjectProperty.

seas:hasProperty a owl:ObjectProperty.

seas:voltage a owl:ObjectProperty.
seas:RNVoltage a owl:ObjectProperty.
seas:SNoltage a owl:ObjectProperty.
seas:TNVoltage a owl:ObjectProperty.

seas:current a owl:ObjectProperty.
seas:rCurrent a owl:ObjectProperty.
seas:sCurrent a owl:ObjectProperty.
seas:tCurrent a owl:ObjectProperty.

seas:consumedElectricEnergy a owl:ObjectProperty.

seas:electricEnergy a owl:ObjectProperty.

fiemser:hasNominalVoltage a owl:DatatypeProperty.

fiemser:hasNominalPower a owl:DatatypeProperty.

fiemser:hasNominalVoltage a owl:DatatypeProperty.